theories/memcpy.v
@@ -22,9 +22,9 @@ Lemma wp_memcpy `{heapG Σ} E l1 l2 vl1 vl2 q n:
   length vl1 = n → length vl2 = n →
   {{{ heap_ctx ∗ l1 ↦∗ vl1 ∗ l2 ↦∗{q} vl2 }}}
     #l1 <-{n} !#l2 @ E
-  {{{; #(), l1 ↦∗ vl2 ∗ l2 ↦∗{q} vl2 }}}.
+  {{{ RET #(); l1 ↦∗ vl2 ∗ l2 ↦∗{q} vl2 }}}.
 Proof.
-  iIntros (? Hvl1 Hvl2 Φ) "[(#Hinv & Hl1 & Hl2) HΦ]".
+  iIntros (? Hvl1 Hvl2 Φ) "(#Hinv & Hl1 & Hl2) HΦ".
   iLöb as "IH" forall (n l1 l2 vl1 vl2 Hvl1 Hvl2). wp_rec. wp_op=> ?; wp_if.
   - iApply "HΦ". assert (n = O) by lia; subst.
     destruct vl1, vl2; try discriminate. by iFrame.
